test.dfy
@@ -1,6 +1,32 @@
 method Main()
 {
-    var a := new int[5];
-    var d := a[0..4];
-    print d;
+    var a := new int[3];
+    a[0] := 1;
+    a[1] := 2;
+    a[2] := 3;
+    var start_a := 0;
+    var size_a := 3;
+
+    var b := new int[3];
+    b[0] := 4;
+    b[1] := 5;
+    b[2] := 6;
+    var start_b := 2;
+    var size_b := 3;
+
+    var s1 := if start_a + size_a <= a.Length
+            then a[start_a..start_a + size_a]
+            else a[start_a..] + a[..start_a - (a.Length - start_a)];
+
+    print s1;
+
+    var s2 := if start_b + size_b <= b.Length
+            then b[start_b..start_b + size_b]
+            else b[start_b..] + b[..start_b - (b.Length - start_b) + 1];
+
+    print s2;
+
+    var s3 := s1 + s2;
+
+    print s3;
 }
